examples/core/Core.Iter.Traits.Collect.fst
@@ -6,7 +6,7 @@ class into_iterator self = {
   f_into_iter: self -> f_IntoIter;
 }
 
-unfold instance impl t {| Core.Iter.iterator t |}: into_iterator t = {
+unfold instance impl t {| Core.Iter.Traits.Iterator.iterator t |}: into_iterator t = {
   f_IntoIter = t;
   f_into_iter = id;
 }
